\documentclass[UTF8]{ctexart}
\usepackage{setspace}
\usepackage{amssymb}
\usepackage[a4paper, total={6.5in, 9.5in}]{geometry}

\begin{document}
%标题
\section*{
  \begin{center}
      \huge
      信息与计算科学导论\\
      Number Theory\\
      221502023 \  沈硕 \  第四次作业\\
  \end{center}
 }

%Problem 38
\subsection*{
    \begin{flushleft}
        \Large
        Problem 38
            [Difficulty Estimate=2.4]
        Prove Proposition 52 without using induction.\\
        Proposition 52:
        For any distinct odd numbers p, q > 1,
        suppose f is the permutation on $Z_{pq}$ that maps
        aq + b to a + bp for every $a \in Z_p, b \in Z_q$.
        Then, f has the same parity as $\frac{(p-1)(q-1)}{4}$.
    \end{flushleft}
}%Solution to Problem 38
\begin{flushleft}
    \Large
    Solution: I give up.
\end{flushleft}

%Problem 39
\subsection*{
    \begin{flushleft}
        \Large
        Problem 39
            [Difficulty Estimate=1.2]
        Prove Propositions 53 and 54.\\
        Proposition 53:
        For any positive odd integers n, m and any integers a, b,
        the Jacobi symbol $(\frac{ab}{n}) =(\frac{a}{n})(\frac{b}{n})$;
        the Jacobi symbol $(\frac{a}{nm})=(\frac{a}{n})(\frac{a}{m})$.
        \\Proposition 54 :
        For any positive odd integers n,
        the Jacobi symbol $(\frac{-1}{n}) = 1$ if $n \equiv 1\ (mod\ 4)$;
        $(\frac{-1}{n})=-1$ if $n \equiv 3\ (mod\ 4)$;
        the Jacobi symbol $(\frac{2}{n}) = 1$ if $n \equiv \pm 1\ (mod\ 8)$;
        $(\frac{2}{n}) = -1$ if $n \equiv \pm 3\ (mod\ 8)$.
    \end{flushleft}
}%Solution to Problem 39
\begin{flushleft}
    \Large
    Solution to Proposition 53:\\
    Denote n as $p_1^{k_1}\cdots p_l^{k_l}$,
    where $p_1 \cdots p_k$ are all odd primes.\\
    $\frac{ab}{n} = (\frac{ab}{p_1})^{k_1} \cdots (\frac{ab}{p_l})^{k_l}$,
    And as the $(\frac{ab}{p_i})^{k_i}$ can also be a Legender symbol,
    so it can be seperated as
    $((\frac{a}{p_i})(\frac{b}{p_i}))^{k_i}$.
    Apply this to all $i = 1,2,\cdots ,l$ can prove the former one.\\
    For the latter one, denote m as $q_1^{i_1}\cdots q_j^{i_j}$,
    then by the definition of Jacobi symbol we can similarly reach the proposition.\\
    Solution to Proposition 54:\\
    $(\frac{-1}{n}) = \prod_{i=1}^{l}(\frac{-1}{x_i})$, $n = x_1 x_2 \cdots x_l$,
    $\Rightarrow (-1)^{\frac{\prod_{i=1}^{l} x_i -1}{2}} = \prod_{i=1}^{l}(-1)^{\frac{x_i-1}{2}}$.
    So $(\frac{-1}{n}) = 1 \Leftrightarrow$ the number of $x_i \equiv 3\ (mod\ 4)$ is even.\\
    $\Leftrightarrow n \equiv 1\ (mod\ 4)$.
    Similar proof to $(\frac{-1}{n})=-1$ if $n \equiv 3\ (mod\ 4)$.\\
    If p is a prime, then $(\frac{2}{p}) = (-1)^{\frac{p^2-1}{8}}$.
    Then $(\frac{2}{n}) = (-1)^{\Sigma_{i=1}^{l}k_i\frac{p_i^2-1}{8}}$\\
    So $(\frac{2}{n}) = 1 \Leftrightarrow$
    the number of $p_i \equiv \pm 3\ (mod\ 8)$ is even.
    $\Leftrightarrow n \equiv 1\ (mod\ 4)$.
    Similar proof to $(\frac{2}{n}) = -1$ if $n \equiv \pm 3\ (mod\ 8)$.
\end{flushleft}

%Problem 40
\subsection*{
    \begin{flushleft}
        \Large
        Problem 40
            [Difficulty Estimate=1.2]
        Read another proof of Gauss quadratic reciprocity.
        For example, you may consider reading the original proof by Gauss,
        or the famous alternative proof by Einstein.
    \end{flushleft}
}%Solution to Problem 40
\begin{flushleft}
    \Large
    Solution: I have read it... That sounds very strange and difficult www.
\end{flushleft}

%Problem 41
\subsection*{
    \begin{flushleft}
        \Large
        Problem 41
            [Difficulty Estimate=1.8]
        Suppose a is a positive integer but not a perfect square
        (i.e., not equal to the square of any integer).
        Prove that there exist infinitely many primes p such that
        $(\frac{a}{p}) = -1$
    \end{flushleft}
}%Solution to Problem 41
\begin{flushleft}
    \Large
    Solution:
    Since a is not a perfect square,
    a can be denoted by $q^k m$,
    where k is an odd integer to satisfy a is not a perfect square,
    and m is a positive integer and coprime to q.\\

    Then $(\frac{a}{p}) = (\frac{q}{p})^k (\frac{m}{p})$
    $=(\frac{q}{p})^k\ \Pi _{i=1}^{n} (\frac{b_i}{p}) ^ {c_i}$,
    where we let $m = \Pi _{i=1}^{n} b_i ^ {c_i}$ and
    $b_i , i=1,2,\cdots,n$ are all primes.\\

    Observed that if
    $(\frac{q}{p}) = -1\ and\ (\frac{b_i}{p}) = 1\ ,\forall i$,
    then $(\frac{a}{p}) = -1$ can be satisfied.\\

    By quadratic reciprocity,
    $(\frac{q}{p})(\frac{p}{q}) = (-1)^{\frac{(p-1)(q-1)}{4}}$,
    and if $p \equiv 1\ (mod\ 4)$, then this quadratic reciprocity leads to
    $(\frac{q}{p})(\frac{p}{q}) = 1$.
    In this situation,$(\frac{q}{p})$ and $(\frac{p}{q})$ are all 1 or -1.
    Then it switches to find p to satisfy $(\frac{p}{q}) = -1$.
    We can arbitrarily choose an x s.t. x is a $QNR_q$,
    then choose p s.t. $p \equiv x\ (mod\ q)$ can make $(\frac{p}{q}) = -1$.\\

    Then consider $(\frac{b_i}{p})(\frac{p}{b_i}) = (-1)^\frac{(p-1)(b_i-1)}{4}$.
    Since $p \equiv 1\ (mod\ 4)$, there must be $(\frac{b_i}{p})(\frac{p}{b_i}) = 1$.
    To make $(\frac{b_i}{p}) = 1$, letting $p \equiv 1\ (mod\ b_i)$ can satisfy.\\

    So, summing up all conditions below:
    $p \equiv 1\ (mod\ 4)$,
    $p \equiv x\ (mod\ q)$,
    $p \equiv 1\ (mod\ b_i)$.
    Denote $b_{n+1} = 4,\ b_{n+2} = q$,
    $Q = Pi _{i=1}^{n+2} b_i$\\
    Using CRT can get
    $p = \sum_{i=1}^{n+1} \frac{Q}{b_i}[\frac{Q}{b_i}]^{-1}
        + x\frac{Q}{q}[\frac{Q}{q}]^{-1} + kQ$.
    And if q or $b_i$ is 2 then delete the correpondent equiv is also well.\\
    $\sum_{i=1}^{n+1} \frac{Q}{b_i}[\frac{Q}{b_i}]^{-1}
        + x\frac{Q}{q}[\frac{Q}{q}]^{-1}$
    is coprime to Q, because for $b_i$,
    $\forall j\neq i,\ b_i \mid Q ,\ b_i \mid \frac{Q}{b_j}[\frac{Q}{b_j}]^{-1}$ ,
    but $b_i \nmid \frac{Q}{b_i}[\frac{Q}{b_i}]^{-1}$.
    So by Dirichlet Lemma there are infinite p.
\end{flushleft}
\end{document}